Simplified example

examples/simple_state_machine.v
@@ -5,30 +5,28 @@ Local Obligation Tactic := idtac.
 
 Inductive State :=
   | initial
-  | one
-  | two
+  | middle
   | extra
   | final
 .
 
 Inductive Transition (before : State) :=
   | advance (prf : before <> final)
-  | sidetrack (prf : before = one).
+  | sidetrack (prf : before = initial).
 
 Local Obligation Tactic := try discriminate.
 Program Definition step (s : State) (t : Transition s) :=
   match t with
   | advance _ _ =>
     match s with
-    | initial => one
-    | one => two
-    | two => final
-    |  extra => two
+    | initial => middle
+    | middle => final
+    | extra => middle
     | final => _
     end
   | sidetrack _ _ =>
     match s with
-    | one => extra
+    | initial => extra
     | _ => _
     end
 end.
@@ -45,23 +43,22 @@ subst.
 contradiction.
 Defined.
 
-Lemma four_transitions_gives_final : 
-  forall t1 t2 t3 t4,
+Lemma three_transitions_gives_final : 
+  forall t1 t2 t3,
   let s1 := step initial t1 in
   let s2 := step s1 t2 in
-  let s3 := step s2 t3 in
-  step s3 t4 = final.
+  step s2 t3 = final.
 Proof.
   intros.
   destruct t1. simpl in *.
-  destruct t2. simpl in *.
-  destruct t3. simpl in *.
-  destruct t4.
-    contradiction.
-    discriminate.
-  discriminate.
-  simpl in *.
-  destruct t3. simpl in *. destruct t4. simpl in *. reflexivity. discriminate.
-  discriminate.
-  discriminate.
+    - destruct t2. simpl in *.
+      + destruct t3.
+        * contradiction.
+        * discriminate.
+      + discriminate. 
+    - destruct t2. simpl in *.
+        + destruct t3. simpl in *.
+          * reflexivity.
+          * discriminate.
+        + discriminate.
 Qed.
